#math #continuity #discontinuous 
# Factoring Method
## Example:
Given the function $f(x) = \frac{6x^2+18x+12}{x^2-4}$, remove the discontinuity at $f(-2)$
### Solution:
Rewrite:
$$f(x)=\frac{6(x^2+3x+2)}{(x+2)(x-2)}=\frac{6(x+1)(x+2)}{(x+2)(x-2)}$$Cancel out like terms:
$$=\frac{6(x+1)}{x-2}\mbox{ for }x\neq-2$$
Determine what the function should be at $-2$ by using [[Limits by Direct Substitution]]: $$lim_{x\rightarrow-2}f(x)=\frac{6((-2)+1)}{(-2)-2}=\frac{-6}{-4}=\frac{3}{2}$$Therefore, to remove the discontinuity: $$f(x)=\frac{6(x+1)}{x-2}\mbox{ for }x\neq-2\mbox{ and }\frac{3}{2}\mbox{ for }x=-2$$

# Rationalization Method
I don't want to do this right now...